generational/spec/GC.Gen.ChunkedCheney.fst
@@ -323,6 +323,27 @@ let chunked_cheney_scan_step
                alloc_fuel))
   = ()
 
+let chunked_cheney_promote_equation
+  (minor: minor_state) (major: MH.major_heap) (fp: U64.t)
+  (roots: seq U64.t) (alloc_fuel: nat)
+  : Lemma
+      (ensures
+        (let cs0 : chunked_cheney_state =
+           { ccs_major = major;
+             ccs_fp = fp;
+             ccs_fwd = empty_forwarding;
+             ccs_queue = Seq.empty } in
+         let cs1 =
+           chunked_cheney_forward_roots minor cs0 roots 0 alloc_fuel in
+         let cs2 =
+           chunked_cheney_scan
+             minor cs1 0 (Dense.cheney_fuel minor) alloc_fuel in
+         chunked_cheney_promote minor major fp roots alloc_fuel ==
+         { major_final = cs2.ccs_major;
+           fp_final = cs2.ccs_fp;
+           fwd_map = cs2.ccs_fwd }))
+  = ()
+
 #push-options "--z3rlimit 5 --fuel 0 --ifuel 0 --split_queries always"
 let chunked_cheney_forward_normal_default_single_chunk_compat
   (minor: minor_state) (cs: Dense.cheney_state) (addr: U64.t)
